Plfl/Arith.lean
@@ -1,0 +1,124 @@
+inductive Tm : Type :=
+  | tru : Tm
+  | fls : Tm
+  | ite : Tm -> Tm -> Tm -> Tm
+  | zro : Tm
+  | suc : Tm -> Tm
+  | prd : Tm -> Tm
+  | iszro : Tm -> Tm
+
+notation "true"  => Tm.tru
+notation "false" => Tm.fls
+notation:60 "if" t₁ "then" t₂ "else" t₃ => Tm.ite t₁ t₂ t₃
+notation "zero"   => Tm.zro
+prefix:70 "succ " => Tm.suc
+prefix:70 "pred " => Tm.prd
+prefix:70 "iszero " => Tm.iszro
+
+inductive Val : Tm → Prop :=
+  | tru  : Val true
+  | fls  : Val false
+  | zro : Val zero
+  | suc {n} : Val n -> Val (succ n)
+
+inductive Step : Tm → Tm → Prop
+  | iftru {t₂ t₃}     : Step (if true then t₂ else t₃) t₂
+  | iffls {t₂ t₃}     : Step (if false then t₂ else t₃) t₃
+  | ite {t₁ t₁' t₂ t₃} : Step t₁ t₁' → Step (if t₁ then t₂ else t₃) (if t₁' then t₂ else t₃)
+  | suc {t t'}        : Step t t' → Step (succ t) (succ t')
+  | prdzro            : Step (pred zero) zero
+  | prdsuc {t}        : Step (pred (succ t)) t
+  | prd {t t'}        : Step t t' → Step (pred t) (pred t')
+  | iszrozro          : Step (iszero zero) true
+  | iszrosuc {t}      : Step t zero → Step (iszero (succ t)) false
+  | iszro {t t'}      : Step t t' → Step (iszero t) (iszero t')
+
+infix:40 " —→ " => Step
+
+theorem sample : ∀ n, n = m ∧ m = 0 → n = 0
+  | n , ⟨hn, hm⟩ => by rw [hn, hm]
+
+/- Theorem: Decidability of one-step evaluation -/
+theorem dec_one_step : t —→ t' ∧ t —→ t'' → t' = t''
+  | ⟨Step.iftru, Step.iftru⟩ => rfl
+  | ⟨Step.iftru, Step.ite _⟩ => by contradiction
+  | ⟨Step.iffls, Step.iffls⟩ => rfl
+  | ⟨Step.iffls, Step.ite _⟩ => by contradiction
+  | ⟨Step.ite _, Step.iftru⟩ => by contradiction
+  | ⟨Step.ite _, Step.iffls⟩ => by contradiction
+  | ⟨Step.ite ht₁, Step.ite ht₁'⟩ => by simp [dec_one_step ⟨ht₁, ht₁'⟩]
+  | ⟨Step.suc ht, Step.suc ht'⟩ => by simp [dec_one_step ⟨ht, ht'⟩]
+  | ⟨Step.prdzro, Step.prdzro⟩ => rfl
+  | ⟨Step.prdzro, Step.prd _⟩ => by contradiction
+  | ⟨Step.prdsuc, Step.prdsuc⟩ => rfl
+  | ⟨Step.prdsuc, Step.prd ht'⟩ => by sorry
+  | ⟨Step.prd ht, Step.prdsuc⟩ => by sorry
+  | ⟨Step.prd ht, Step.prd ht'⟩ => by simp [dec_one_step ⟨ht, ht'⟩]
+  | ⟨Step.iszrozro, Step.iszrozro⟩ => rfl
+  | ⟨Step.iszrozro, Step.iszro _⟩ => by contradiction
+  | ⟨Step.iszrosuc _, Step.iszrosuc _⟩ => rfl
+  | ⟨Step.iszrosuc ht, Step.iszro ht'⟩ => by sorry
+  | ⟨Step.iszro ht, Step.iszrosuc ht'⟩ => by sorry
+  | ⟨Step.iszro ht, Step.iszro ht'⟩ => by simp [dec_one_step ⟨ht, ht'⟩]
+
+/- Definition: Normal form -/
+def is_norm (t : Tm) : Prop := ∀ t', ¬ t —→ t'
+
+/- Theorem: All values are normal form -/
+def val_is_norm : ∀ {t}, Val t → is_norm t
+  | true , _ => by simp [is_norm]; intros t h; contradiction
+  | false, _ => by simp [is_norm]; intros t h; contradiction
+  | zero , _ => by simp [is_norm]; intros t h; contradiction
+  | succ n, Val.suc hn => by
+      simp [is_norm]; intros t h;
+      cases h with
+      | @suc _ t' h =>
+          have p := val_is_norm hn
+          simp [is_norm] at p
+          have p' := p t'
+          contradiction
+
+def norm_is_val : ∀ {t}, is_norm t → Val t
+  | true , hn => Val.tru
+  | false, hn => Val.fls
+  | Tm.ite t₁ t₂ t₃, hn => by simp [is_norm] at hn; sorry
+  | zero , hn => Val.zro
+  | succ n, hn => Val.suc (norm_is_val (by simp [is_norm] at *; sorry))
+  | pred n, hn => by simp [is_norm] at hn; sorry
+  | iszero n, hn => sorry
+
+/- Definition: Reflexive and transitive closure of Step -/
+inductive Steps : Tm → Tm → Prop
+  | single : t —→ t' → Steps t t'
+  | refl   : ∀ t, Steps t t
+  | trans  : Steps t t' → Steps t' t'' → Steps t t''
+
+infix:40 " —→* " => Steps
+
+/- Theorem: Uniqueness of normalform -/
+theorem uniq_norm : t —→* u → t —→* u' → is_norm u → is_norm u' → u = u' := by
+  intros ht ht' hn hn'
+  simp [is_norm] at hn hn'
+  induction ht generalizing u' with
+  | single h => induction ht' generalizing u with
+      | single h' => simp [dec_one_step ⟨h, h'⟩]
+      | refl => sorry
+      | trans h₁ h₂ => sorry
+  | refl => sorry
+  | trans h₁ h₂ => sorry
+
+/- Theorem: Termination of evaluation -/
+theorem terminate_steps : ∀ t, ∃ t', is_norm t' ∧ t —→* t' := by
+  intro t
+  induction t with
+  | tru => sorry
+  | fls => exact ⟨false, Steps.refl _⟩
+  | ite t₁ t₂ t₃ =>
+      induction t₁ with
+      | tru => exact ⟨t₂, Steps.single Step.iftru⟩
+      | fls => exact ⟨t₃, Steps.single Step.iffls⟩
+      | _ => sorry
+  | zro => exact ⟨zero, Steps.refl _⟩
+  | suc t => sorry
+  | prd t => sorry
+  | iszro t => sorry
